added Prim (admit)

coq/full/Lambda.v
@@ -44,7 +44,7 @@ Definition eval_km {L : Type} {M : LabelAlgebra unit L} :
                 | TVar n =>
                   exists v l,
                     atIndex e n = Some (Atom v l) /\
-                    a = Atom v (l ⊔ pc)
+                    a = Atom v l
                 | TAbs t' =>
                   a = Atom (VClos e t') pc
                 | TApp t1 t2 =>
@@ -54,6 +54,13 @@ Definition eval_km {L : Type} {M : LabelAlgebra unit L} :
                          eval l P pc e t1 (Atom (VClos e1' t1') l1) /\
                          eval l P pc e t2 a2 /\
                          eval l P l1 (a2 :: e1') t1' a
+                | TPrim f t1 t2 =>
+                  if Compare_dec.zerop (fst km) then False
+                  else let eval := eval_km (fst km - 1, snd km) _ in
+                       exists n1 l1 n2 l2,
+                         eval l P pc e t1 (Atom (VNat L n1) l1) /\
+                         eval l P pc e t2 (Atom (VNat L n2) l2) /\
+                         a = Atom (VNat L (f n1 n2)) (l1 ⊔ l2)
                 | TRelabel t' l' =>
                   if Compare_dec.zerop (fst km) then False
                   else let eval := eval_km (fst km - 1, snd km) _ in
@@ -94,7 +101,7 @@ Lemma eval_km_eq {L : Type} {M : LabelAlgebra unit L} :
         | TVar n =>
           exists v l,
             atIndex e n = Some (Atom v l) /\
-            a = Atom v (l ⊔ pc)
+            a = Atom v l
         | TAbs t' =>
           a = Atom (VClos e t') pc
         | TApp t1 t2 =>
@@ -104,22 +111,29 @@ Lemma eval_km_eq {L : Type} {M : LabelAlgebra unit L} :
                  eval l P pc e t1 (Atom (VClos e1' t1') l1) /\
                  eval l P pc e t2 a2 /\
                  eval l P l1 (a2 :: e1') t1' a
-        | TRelabel t' l' =>
+        | TPrim f t1 t2 =>
           if Compare_dec.zerop (fst km) then False
           else let eval := eval_km (fst km - 1, snd km) in
-               exists v l1,
-                 eval l P pc e t' (Atom v l1) /\
-                 ((l1 ⊑ l' /\
-                   a = Atom v l') \/
-                  (l' ⊑ l1 /\
-                   let eval := eval_km (snd km, fst km - 1) in
-                   (forall pc' e' v' l1',
-                      lab_Lequiv L M l pc pc' ->
-                      env_LPequiv L M l P e e' ->
-                      lab_Lequiv L M l l1 l1' ->
-                      eval l P pc' e' t' (Atom v' l1') ->
-                      value_LPequiv L M l P v v') /\
-                   a = Atom v l'))
+               exists n1 l1 n2 l2,
+                 eval l P pc e t1 (Atom (VNat L n1) l1) /\
+                 eval l P pc e t2 (Atom (VNat L n2) l2) /\
+                 a = Atom (VNat L (f n1 n2)) (l1 ⊔ l2)
+                | TRelabel t' l' =>
+                  if Compare_dec.zerop (fst km) then False
+                  else let eval := eval_km (fst km - 1, snd km) in
+                       exists v l1,
+                         eval l P pc e t' (Atom v l1) /\
+                         ((l1 ⊑ l' /\
+                           a = Atom v l') \/
+                          (l' ⊑ l1 /\
+                           let eval := eval_km (snd km, fst km - 1) in
+                           (forall pc' e' v' l1',
+                              lab_Lequiv L M l pc pc' ->
+                              env_LPequiv L M l P e e' ->
+                              lab_Lequiv L M l l1 l1' ->
+                              eval l P pc' e' t' (Atom v' l1') ->
+                              value_LPequiv L M l P v v') /\
+                           a = Atom v l'))
         | TIf t1 t2 t3 =>
           if Compare_dec.zerop (fst km) then False
           else let eval := eval_km (fst km - 1, snd km) in
@@ -148,6 +162,11 @@ Proof.
     apply functional_extensionality_ex; intro t1'.
     apply functional_extensionality_ex; intro l1.
     apply functional_extensionality_ex; intro a2.
+    rewrite H'. reflexivity.
+  - apply functional_extensionality_ex; intro n1.
+    apply functional_extensionality_ex; intro l1.
+    apply functional_extensionality_ex; intro n2.
+    apply functional_extensionality_ex; intro l2.
     rewrite H'. reflexivity.
   - apply functional_extensionality_ex; intro v.
     apply functional_extensionality_ex; intro l1.
@@ -180,7 +199,7 @@ Proof. intros. rewrite eval_km_eq in H. auto. Qed.
 Lemma eval_km_var {L : Type} {M : LabelAlgebra unit L} :
   forall k m l P pc e n v' l',
     atIndex e n = Some (Atom v' l') ->
-    eval_km (k, m) l P pc e (TVar L n) (Atom v' (l' ⊔ pc)).
+    eval_km (k, m) l P pc e (TVar L n) (Atom v' l').
 Proof. intros. rewrite eval_km_eq. exists v' l'. auto. Qed.
 
 Lemma eval_km_var_inv {L : Type} {M : LabelAlgebra unit L} :
@@ -188,7 +207,7 @@ Lemma eval_km_var_inv {L : Type} {M : LabelAlgebra unit L} :
     eval_km (k, m) l P pc e (TVar L n) a ->
     exists v' l',
       atIndex e n = Some (Atom v' l') /\
-      a = Atom v' (l' ⊔ pc).
+      a = Atom v' l'.
 Proof. intros. rewrite eval_km_eq in H. auto. Qed.
 
 Lemma eval_km_abs {L : Type} {M : LabelAlgebra unit L} :
@@ -230,6 +249,37 @@ Proof.
   - destruct H as [e1' [t1' [l1 [a2 [H1 [H2 H3]]]]]].
     replace (k - 0) with k in * by omega.
     exists k e1' t1' l1 a2. auto.
+Qed.
+
+Lemma eval_km_prim {L : Type} {M : LabelAlgebra unit L} :
+  forall k m l P pc e f t1 t2 n1 l1 n2 l2,
+    eval_km (k, m) l P pc e t1 (Atom (VNat L n1) l1) ->
+    eval_km (k, m) l P pc e t2 (Atom (VNat L n2) l2) ->
+    eval_km (S k, m) l P pc e (TPrim f t1 t2)
+            (Atom (VNat L (f n1 n2)) (l1 ⊔ l2)).
+Proof.
+  intros.
+  rewrite eval_km_eq. simpl.
+  replace (k - 0) with k by omega.
+  exists n1 l1 n2 l2. auto.
+Qed.
+
+Lemma eval_km_prim_inv {L : Type} {M : LabelAlgebra unit L} :
+  forall k m l P pc e f t1 t2 a,
+    eval_km (k, m) l P pc e (TPrim f t1 t2) a ->
+    exists k' n1 l1 n2 l2,
+      k = S k' /\
+      eval_km (k', m) l P pc e t1 (Atom (VNat L n1) l1) /\
+      eval_km (k', m) l P pc e t2 (Atom (VNat L n2) l2) /\
+      a = Atom (VNat L (f n1 n2)) (l1 ⊔ l2).
+Proof.
+  intros.
+  rewrite eval_km_eq in H.
+  destruct k; simpl in H.
+  - inversion H.
+  - destruct H as [n1 [l1 [n2 [l2 [H1 [H2 H3]]]]]].
+    replace (k - 0) with k in * by omega.
+    exists k n1 l1 n2 l2. auto.
 Qed.
 
 Lemma eval_km_relabel_up {L : Type} {M : LabelAlgebra unit L} :
