coq/full/LambdaSyntax.v
@@ -10,6 +10,7 @@ Inductive term (L : Type) : Type :=
   | TVar : nat -> term L
   | TAbs : term L -> term L
   | TApp : term L -> term L -> term L
+  | TPrim : (nat -> nat -> nat) -> term L -> term L -> term L
   | TRelabel : term L -> L -> term L
   | TIf : term L -> term L -> term L -> term L.
 
